@prefix : <http://www.semanticweb.org/lucia/ontologies/2023/0/cdmontology#> .
@prefix owl: <http://www.w3.org/2002/07/owl#> .
@prefix rdf: <http://www.w3.org/1999/02/22-rdf-syntax-ns#> .
@prefix xml: <http://www.w3.org/XML/1998/namespace> .
@prefix xsd: <http://www.w3.org/2001/XMLSchema#> .
@prefix rdfs: <http://www.w3.org/2000/01/rdf-schema#> .
@base <http://www.semanticweb.org/lucia/ontologies/2023/0/cdmontology> .

<http://www.semanticweb.org/lucia/ontologies/2023/0/cdmontology> rdf:type owl:Ontology .

#################################################################
#    Annotation properties
#################################################################

###  http://www.w3.org/2004/02/skos/core#narrower
<http://www.w3.org/2004/02/skos/core#narrower> rdf:type owl:AnnotationProperty .


###  http://www.w3.org/2004/02/skos/core#related
<http://www.w3.org/2004/02/skos/core#related> rdf:type owl:AnnotationProperty .


#################################################################
#    Classes
#################################################################

###  http://www.semanticweb.org/lucia/ontologies/2023/0/cdmontology#Biomass
:Biomass rdf:type owl:Class ;
         rdfs:comment """Non-fossilized and biodegradable organic material originating from plants, animals and micro-organisms, including:
(a) Biomass residue;
(b) The non-fossilized and biodegradable organic fractions of industrial and municipal wastes; and
(c) The gases and liquids recovered from the decomposition of non-fossilized and biodegradable organic
material."""@en .


###  http://www.semanticweb.org/lucia/ontologies/2023/0/cdmontology#CPA
:CPA rdf:type owl:Class ;
     rdfs:label "CPA Project Activity"@en .


###  http://www.semanticweb.org/lucia/ontologies/2023/0/cdmontology#above-groundBiomass
:above-groundBiomass rdf:type owl:Class ;
                     rdfs:subClassOf :Biomass ;
                     owl:disjointWith :below-groundBiomass ;
                     rdfs:comment "All living biomass above the soil including stem, stump, branches, bark, seeds, and foliage as well as herbaceous vegetation."@en .


###  http://www.semanticweb.org/lucia/ontologies/2023/0/cdmontology#additional
:additional rdf:type owl:Class ;
            rdfs:comment """For a CDM project activity (non-A/R) or CPA (non-A/R), the effect of the CDM project activity or CPA to reduce anthropogenic GHG emissions below the level that would have occurred in the absence of the CDM project activity or CPA; or
For an A/R or SSC CPA (A/R), the effect of the A/R or SSC A/R CDM project activity or CPA (A/R) to increase actual net GHG removals by sinks above the sum of the changes in carbon stocks in the carbon pools within the project boundary that would have occurred in the absence of the A/R or SSC CPA (A/R).
Whether or not a CDM project activity or CPA is additional is determined in accordance with the CDM rules and requirements."""@en ;
            <http://www.w3.org/2004/02/skos/core#narrower> <http://www.semanticweb.org/lucia/ontologies/2023/0/aia#Output> .


###  http://www.semanticweb.org/lucia/ontologies/2023/0/cdmontology#afforestation
:afforestation rdf:type owl:Class ;
               rdfs:comment "The direct human-induced conversion of land that has not been forested for a period of at least 50 years to forested land through planting, seeding and/or the human-induced promotion of natural seed sources."@en ;
               <http://www.w3.org/2004/02/skos/core#narrower> <http://www.semanticweb.org/lucia/ontologies/2023/0/aia#Activity> .


###  http://www.semanticweb.org/lucia/ontologies/2023/0/cdmontology#agroforestry
:agroforestry rdf:type owl:Class ;
              rdfs:comment "Growing of both trees and agricultural / horticultural crops on the same piece of land."@en ;
              <http://www.w3.org/2004/02/skos/core#narrower> <http://www.semanticweb.org/lucia/ontologies/2023/0/aia#Activity> .


###  http://www.semanticweb.org/lucia/ontologies/2023/0/cdmontology#allometricBiomassEquations
:allometricBiomassEquations rdf:type owl:Class ;
                            rdfs:comment "Regression equations calculating biomass based on measured parameters of a tree (or shrub), for example, quantifying the relationship between above-ground tree biomass and the diameter at breast height and tree height of a specific tree species."@en .


###  http://www.semanticweb.org/lucia/ontologies/2023/0/cdmontology#baselineScenario
:baselineScenario rdf:type owl:Class ;
                  rdfs:comment """For a CDM project activity (non-A/R) or CPA (non-A/R), the scenario for a CDM project activity or CPA that reasonably represents the anthropogenic emissions by sources of GHG that would occur in the absence of the proposed CDM project activity or CPA.
For an A/R or SSC A/R CDM project activity or CPA (A/R), the scenario for an A/R or SSC A/R CDM project activity or CPA (A/R) that reasonably represents the sum of the changes in carbon stocks in the carbon pools within the project boundary that would occur in the absence of the A/R or SSC A/R CDM project activity or CPA (A/R)."""@en ;
                  <http://www.w3.org/2004/02/skos/core#related> <http://www.semanticweb.org/lucia/ontologies/2023/0/aia#State> .


###  http://www.semanticweb.org/lucia/ontologies/2023/0/cdmontology#below-groundBiomass
:below-groundBiomass rdf:type owl:Class ;
                     rdfs:subClassOf :Biomass ;
                     rdfs:comment "All living biomass of roots. Fine roots of less than (suggested) 2 mm diameter are often excluded because these often cannot be distinguished empirically from soil organic matter or litter."@en .


###  http://www.semanticweb.org/lucia/ontologies/2023/0/cdmontology#biomassExpansionFactor
:biomassExpansionFactor rdf:type owl:Class ;
                        rdfs:comment "Ratio of total stand biomass to stand (merchantable) volume (e.g. as derived from forest yield tables)."@en .


###  http://www.semanticweb.org/lucia/ontologies/2023/0/cdmontology#captiveGeneration
:captiveGeneration rdf:type owl:Class ;
                   rdfs:comment "Electricity generation in a power plant that supplies electricity only to consumer(s) and not to the electricity grid. The consumer(s) are either located directly at the site of the power plant or are connected through dedicated electricity distribution line(s) with the power plant but not via the electricity grid."@en ;
                   <http://www.w3.org/2004/02/skos/core#narrower> <http://www.semanticweb.org/lucia/ontologies/2023/0/aia#Activity> .


###  http://www.semanticweb.org/lucia/ontologies/2023/0/cdmontology#carbonSequestration
:carbonSequestration rdf:type owl:Class ;
                     rdfs:comment "Carbon sequestration is defined as a biological, chemical or physical process of removing carbon from the atmosphere and depositing it in a reservoir."@en ;
                     <http://www.w3.org/2004/02/skos/core#narrower> <http://www.semanticweb.org/lucia/ontologies/2023/0/aia#Activity> .


###  http://www.semanticweb.org/lucia/ontologies/2023/0/cdmontology#cogeneration
:cogeneration rdf:type owl:Class ;
              rdfs:comment "Simultaneous production of electricity and useful thermal energy in one process."@en ;
              <http://www.w3.org/2004/02/skos/core#narrower> <http://www.semanticweb.org/lucia/ontologies/2023/0/aia#Activity> .


###  http://www.semanticweb.org/lucia/ontologies/2023/0/cdmontology#non-renewableBiomass
:non-renewableBiomass rdf:type owl:Class ;
                      rdfs:subClassOf :Biomass ;
                      owl:disjointWith :renewableBiomass ;
                      rdfs:comment "Biomass not fulfilling the conditions of renewable biomass is considered as non-renewable."@en .


###  http://www.semanticweb.org/lucia/ontologies/2023/0/cdmontology#renewableBiomass
:renewableBiomass rdf:type owl:Class ;
                  rdfs:subClassOf :Biomass ;
                  rdfs:comment """Biomass which meets one of the following conditions:
(a) The biomass originates from land areas that are forests where:
(i) The land area remains a forest;
(ii) Sustainable management practices are undertaken on these land areas to ensure, in particular, that
the level of carbon stocks on these land areas does not systematically decrease over time (carbon
stocks may temporarily decrease due to harvesting); and
(iii) Any national or regional forestry and nature conservation regulations are complied with;
(b) The biomass is woody biomass and originates from croplands and/or grasslands where:
(i) The land area remains cropland and/or grasslands or is reverted to forest; and
(ii) Sustainable management practices are undertaken on these land areas to ensure in particular that
the level of carbonstocks on these land areas does not systematically decrease over time (carbon
stocks may temporarily decrease due to harvesting); and
(iii) Any national or regional forestry, agriculture and nature conservation regulations are complied with;
(c) The biomass is non-woody biomass and originates from croplands and/or grasslands where:
(i) The land area remains cropland and/or grasslands or is reverted to forest; and
(ii) Sustainable management practices are undertaken on these land areas to ensure in particular that
the level of carbon stocks on these land areas does not systematically decrease over time (carbon
stocks may temporarily decrease due to harvesting); and
(iii) Any national or regional forestry, agriculture and nature conservation regulations are complied with;
(d) The biomass is a biomass residue and the use of that biomass residue in the CDM project activity (A/R) does not involve a decrease of carbon pools, in particular dead wood, litter or soil organic carbon, on the land areas from which the biomass residues originate;
(e) The biomass is the non-fossil fraction of an industrial or municipal waste."""@en .


###  http://www.semanticweb.org/lucia/ontologies/2023/0/cdmontology#residueBiomass
:residueBiomass rdf:type owl:Class ;
                rdfs:subClassOf :Biomass .


###  http://www.semanticweb.org/lucia/ontologies/2023/0/cdmontology#A/R
<http://www.semanticweb.org/lucia/ontologies/2023/0/cdmontology#A/R> rdf:type owl:Class ;
                                                                     rdfs:subClassOf :CPA ;
                                                                     rdfs:label "Afforestation/reforestation activity"@en .


###  Generated by the OWL API (version 4.5.9.2019-02-01T07:24:44Z) https://github.com/owlcs/owlapi
